src/sys_verif/assignment3/infer_specs.v
@@ -1,0 +1,74 @@
+
+(*| ## Assignment 3: Inferring specifications
+
+For each `Example` function in [go/heap/exercises.go](https://github.com/tchajed/sys-verif-fa24-proofs/blob/main/go/heap/exercises.go), come up with a general specification of the snippet's behavior, state it in Coq, and prove it correct. A specification for `ExampleA` is provided below as an example.
+
+|*)
+
+From sys_verif Require Import prelude empty_ffi.
+From Goose.sys_verif_code Require Import heap.
+
+Section goose.
+Context `{!heapGS Σ}.
+
+(* worked example of a general specification *)
+Lemma wp_ExampleA (x_l y_l: loc) (z: w64) (x: bool) (y: w64) q :
+  {{{ "x" :: x_l ↦[boolT]{q} #x ∗ "y" :: y_l ↦[uint64T] #y }}}
+    ExampleA #x_l #y_l #z
+  {{{ RET #(); x_l ↦[boolT]{q} #x ∗
+               y_l ↦[uint64T] (if x then #z else #0) }}}.
+Proof.
+  wp_start as "H". iNamed "H".
+Admitted.
+
+Lemma wp_ExampleB :
+  {{{ True }}}
+    ExampleB #()
+  {{{ RET #(); True }}}.
+Proof.
+  (* FILL IN HERE *)
+Admitted.
+
+Lemma wp_ExampleC :
+  {{{ True }}}
+    ExampleC #()
+  {{{ RET #(); True }}}.
+Proof.
+  (* FILL IN HERE *)
+Admitted.
+
+(*| **Warning**: this one is a bit harder than the rest in both specification and proof. |*)
+Lemma wp_ExampleD :
+  {{{ True }}}
+    ExampleD #()
+  {{{ RET #(); True }}}.
+Proof.
+  (* FILL IN HERE *)
+Admitted.
+
+(* you will not need to directly use this, it will be used automatically *)
+Lemma slice_nil_ty ty : val_ty slice.nil (slice.T ty).
+Proof.
+  change slice.nil with (slice_val Slice.nil).
+  apply slice_val_ty.
+Qed.
+
+Hint Resolve slice_nil_ty : core.
+
+Lemma wp_ExampleE :
+  {{{ True }}}
+    ExampleE #()
+  {{{ RET #(); True }}}.
+Proof.
+  (* FILL IN HERE *)
+Admitted.
+
+(*| **Hint:** you can check `exercises_test.go` file to figure out what this function does. |*)
+Lemma wp_ExampleG :
+  {{{ True }}}
+    ExampleG #()
+  {{{ RET #(); True }}}.
+Proof.
+  (* FILL IN HERE *)
+Admitted.
+End goose.
