src/sys_verif/assignment3/linked_list_proof.v
@@ -1,0 +1,110 @@
+(*| # Linked lists
+
+This proof develops a specification for the linked-list implementation at
+[go/heap/linked_list.go](https://github.com/tchajed/sys-verif-fa24-proofs/blob/main/go/heap/linked_list.go).
+
+You should start by reading the Go code.
+
+The idea of this proof is similar to what you saw in Assignment 2's exercise 5,
+but with the code written in Go (and thus using nil pointers rather than an
+inductive data type) and with the proof written in Coq (so you have the Iris
+Proof Mode rather than writing a proof outline).
+
+|*)
+From sys_verif.program_proof Require Import prelude.
+From Goose.sys_verif_code Require Import heap.
+
+
+Section proof.
+Context `{hG: heapGS Σ, !ffi_semantics _ _, !ext_types _}.
+
+(* We abbreviate "linked list" to "ll" in some of these definitions to keep
+specs and other theorem statements concise. *)
+
+(*| After reading the code, read the definition of `ll_rep` and understand how it relates a list pointer (which will be a `n *Node`) to a list of values `xs: list w64`. |*)
+
+Fixpoint ll_rep (l: loc) (xs: list w64) : iProp Σ :=
+  match xs with
+  | nil => "%Heq" :: ⌜l = null⌝
+  | cons x xs' => (∃ (next_l: loc),
+      "elem" :: l ↦[Node :: "elem"] #x ∗
+      "next" :: l ↦[Node :: "next"] #next_l ∗
+      "Hnext_l" :: ll_rep next_l xs')%I
+  end.
+
+(*| The proofs will work by analysis on `xs`, but the code checks if `l` is `nil`
+or not. We relate the two with the following two lemmas (note that the Gallina `null` is the
+model of the Go `nil` pointer). |*)
+
+Definition ll_rep_null l :
+  ll_rep l [] -∗ ⌜l = null⌝.
+Proof.
+  simpl. auto.
+Qed.
+
+Definition ll_rep_non_null l x xs :
+  ll_rep l (x::xs) -∗ ⌜l ≠ null⌝.
+Proof.
+  simpl. iIntros "H". iNamed "H".
+  iDestruct (struct_field_pointsto_not_null with "elem") as %Hnot_null.
+  { reflexivity. }
+  { simpl. lia. }
+  auto.
+Qed.
+
+(*| Prove this specification. |*)
+Lemma wp_NewList :
+  {{{ True }}}
+    NewList #()
+  {{{ (l: loc), RET #l; ll_rep l [] }}}.
+Proof.
+Admitted.
+
+
+(*| Fill in a postcondition here and prove this specification. |*)
+Lemma wp_Node__Insert (l: loc) (xs: list w64) (elem: w64) :
+  {{{ ll_rep l xs }}}
+    Node__Insert #l #elem
+  {{{ (l': loc), RET #l';
+      False  }}}.
+Proof.
+Admitted.
+
+(*| Prove this specification. |*)
+Lemma wp_Node__Pop (l: loc) (xs: list w64) :
+  {{{ ll_rep l xs }}}
+    Node__Pop #l
+  {{{ (x: w64) (l': loc) (ok: bool), RET (#x, #l', #ok);
+      if ok then ∃ xs', ⌜xs = cons x xs'⌝ ∗
+                        ll_rep l' xs'
+      else ⌜xs = []⌝
+  }}}.
+Proof.
+Admitted.
+
+
+(*| Fill in this specification. (You should read the code to see what it does and how it manages the memory of the two lists.)
+
+A general structure is provided for the proof (which you are allowed to change if you find it helpful); fill in the rest of the proof.
+|*)
+Lemma wp_Node__Append l1 xs1 l2 xs2 :
+  {{{ ll_rep l1 xs1 ∗ ll_rep l2 xs2 }}}
+    Node__Append #l1 #l2
+  {{{ (l2': loc), RET #l2';
+      False  }}}.
+Proof.
+  generalize dependent xs2.
+  generalize dependent l2.
+  generalize dependent l1.
+  induction xs1 as [|x1 xs1 IH_wp_Append].
+  - intros l1 l2 xs2. wp_start as "[Hl1 Hl2]".
+    iDestruct (ll_rep_null with "Hl1") as %Hnull.
+    admit.
+  - intros l1 l2 xs2. wp_start as "[Hl1 Hl2]".
+    (* Notice the hypothesis `IH_wp_Append`, which is available due to the use
+    of `induction`. You'll need it to reason about the recursive call. *)
+    iDestruct (ll_rep_non_null with "Hl1") as %Hnull.
+    admit.
+Admitted.
+
+End proof.
